some refactoring

examples/dsls/mini_steel/Pulse.Checker.fsti
@@ -12,11 +12,14 @@ val check_tot (f:RT.fstar_top_env) (g:env) (t:term)
   : T.Tac (_:(ty:pure_term &
               src_typing f g t (C_Tot ty)) { is_pure_term t })
 
-val check (f:RT.fstar_top_env)
-          (g:env)
-          (t:term)
-          (pre:pure_term)
-          (pre_typing: tot_typing f g pre Tm_VProp)
-          (post_hint:option term)
-  : T.Tac (c:pure_comp { C_ST? c ==> comp_pre c == pre } &
-           src_typing f g t c)
+type check_t =
+  f:RT.fstar_top_env ->
+  g:env ->
+  t:term ->
+  pre:pure_term ->
+  pre_typing:tot_typing f g pre Tm_VProp ->
+  post_hint:option term ->
+  T.Tac (c:pure_comp{C_ST? c ==> comp_pre c == pre} &
+         src_typing f g t c)
+
+val check : check_t
